semantics/prop/vyperTypeContractPropsScript.sml
@@ -322,3 +322,554 @@ Proof
   irule build_contract_type_artifact_fn_sigs_complete >>
   simp[]
 QED
+
+
+(* ===== Static-map soundness bridges for contract artifacts ===== *)
+
+Theorem add_toplevel_static_maps_toplevel_vtypes_sound:
+  FLOOKUP (add_toplevel_static_maps F src tl art).cta_toplevel_vtypes k = SOME vt ==>
+  FLOOKUP art.cta_toplevel_vtypes k = SOME vt \/
+  (?vis mut id ty init.
+     tl = VariableDecl vis mut id ty init /\
+     k = (src,string_to_num id) /\ vt = Type ty) \/
+  (?vis is_transient id kt vty init.
+     tl = HashMapDecl vis is_transient id kt vty init /\
+     k = (src,string_to_num id) /\ vt = HashMapT kt vty)
+Proof
+  Cases_on `tl` >>
+  rw[add_toplevel_static_maps_def, FLOOKUP_UPDATE] >>
+  TRY (Cases_on `v0` >> gvs[add_toplevel_static_maps_def, FLOOKUP_UPDATE]) >>
+  gvs[add_toplevel_static_maps_def, FLOOKUP_UPDATE] >>
+  gvs[AllCaseEqs()] >> metis_tac[]
+QED
+
+Theorem add_toplevel_static_maps_bare_globals_sound:
+  FLOOKUP (add_toplevel_static_maps F src tl art).cta_bare_globals k = SOME ty ==>
+  FLOOKUP art.cta_bare_globals k = SOME ty \/
+  (?vis id typ init.
+     tl = VariableDecl vis Immutable id typ init /\
+     k = (src,string_to_num id) /\ ty = typ) \/
+  (?vis e id typ init.
+     tl = VariableDecl vis (Constant e) id typ init /\
+     k = (src,string_to_num id) /\ ty = typ)
+Proof
+  Cases_on `tl` >>
+  rw[add_toplevel_static_maps_def, FLOOKUP_UPDATE] >>
+  TRY (Cases_on `v0` >> gvs[add_toplevel_static_maps_def, FLOOKUP_UPDATE]) >>
+  gvs[add_toplevel_static_maps_def, FLOOKUP_UPDATE] >>
+  gvs[AllCaseEqs()] >> metis_tac[]
+QED
+
+Theorem add_toplevel_static_maps_bare_global_assignable_sound:
+  FLOOKUP (add_toplevel_static_maps F src tl art).cta_bare_global_assignable k = SOME ty ==>
+  FLOOKUP art.cta_bare_global_assignable k = SOME ty \/
+  ?vis id typ init.
+    tl = VariableDecl vis Immutable id typ init /\
+    k = (src,string_to_num id) /\ ty = typ
+Proof
+  Cases_on `tl` >>
+  rw[add_toplevel_static_maps_def, FLOOKUP_UPDATE] >>
+  TRY (Cases_on `v0` >> gvs[add_toplevel_static_maps_def, FLOOKUP_UPDATE]) >>
+  gvs[add_toplevel_static_maps_def, FLOOKUP_UPDATE] >>
+  gvs[AllCaseEqs()] >> metis_tac[]
+QED
+
+Theorem add_toplevel_static_maps_flag_members_sound:
+  FLOOKUP (add_toplevel_static_maps F src tl art).cta_flag_members k = SOME members ==>
+  FLOOKUP art.cta_flag_members k = SOME members \/
+  ?fid ls.
+    tl = FlagDecl fid ls /\ k = (src,fid) /\ members = ls
+Proof
+  Cases_on `tl` >>
+  rw[add_toplevel_static_maps_def, FLOOKUP_UPDATE] >>
+  TRY (Cases_on `v0` >> gvs[add_toplevel_static_maps_def, FLOOKUP_UPDATE]) >>
+  gvs[add_toplevel_static_maps_def, FLOOKUP_UPDATE] >>
+  gvs[AllCaseEqs()] >> metis_tac[]
+QED
+
+Theorem add_module_static_maps_toplevel_vtypes_sound:
+  FLOOKUP (add_module_static_maps F src tls art).cta_toplevel_vtypes k = SOME vt ==>
+  FLOOKUP art.cta_toplevel_vtypes k = SOME vt \/
+  (?tl vis mut id ty init.
+     MEM tl tls /\ tl = VariableDecl vis mut id ty init /\
+     k = (src,string_to_num id) /\ vt = Type ty) \/
+  (?tl vis is_transient id kt vty init.
+     MEM tl tls /\ tl = HashMapDecl vis is_transient id kt vty init /\
+     k = (src,string_to_num id) /\ vt = HashMapT kt vty)
+Proof
+  qid_spec_tac `art` >> Induct_on `tls` >- rw[add_module_static_maps_def] >>
+  rw[add_module_static_maps_def] >>
+  first_x_assum (qspec_then `add_toplevel_static_maps F src h art` mp_tac) >>
+  simp[add_module_static_maps_def] >> strip_tac >-
+    (drule add_toplevel_static_maps_toplevel_vtypes_sound >> rw[] >> gvs[] >> metis_tac[]) >>
+  metis_tac[]
+QED
+
+Theorem add_module_static_maps_bare_globals_sound:
+  FLOOKUP (add_module_static_maps F src tls art).cta_bare_globals k = SOME ty ==>
+  FLOOKUP art.cta_bare_globals k = SOME ty \/
+  (?tl vis id typ init.
+     MEM tl tls /\ tl = VariableDecl vis Immutable id typ init /\
+     k = (src,string_to_num id) /\ ty = typ) \/
+  (?tl vis e id typ init.
+     MEM tl tls /\ tl = VariableDecl vis (Constant e) id typ init /\
+     k = (src,string_to_num id) /\ ty = typ)
+Proof
+  qid_spec_tac `art` >> Induct_on `tls` >- rw[add_module_static_maps_def] >>
+  rw[add_module_static_maps_def] >>
+  first_x_assum (qspec_then `add_toplevel_static_maps F src h art` mp_tac) >>
+  simp[add_module_static_maps_def] >> strip_tac >-
+    (drule add_toplevel_static_maps_bare_globals_sound >> rw[] >> gvs[] >> metis_tac[]) >>
+  metis_tac[]
+QED
+
+Theorem add_module_static_maps_bare_global_assignable_sound:
+  FLOOKUP (add_module_static_maps F src tls art).cta_bare_global_assignable k = SOME ty ==>
+  FLOOKUP art.cta_bare_global_assignable k = SOME ty \/
+  ?tl vis id typ init.
+    MEM tl tls /\ tl = VariableDecl vis Immutable id typ init /\
+    k = (src,string_to_num id) /\ ty = typ
+Proof
+  qid_spec_tac `art` >> Induct_on `tls` >- rw[add_module_static_maps_def] >>
+  rw[add_module_static_maps_def] >>
+  first_x_assum (qspec_then `add_toplevel_static_maps F src h art` mp_tac) >>
+  simp[add_module_static_maps_def] >> strip_tac >-
+    (drule add_toplevel_static_maps_bare_global_assignable_sound >> rw[] >> gvs[] >> metis_tac[]) >>
+  metis_tac[]
+QED
+
+Theorem add_module_static_maps_flag_members_sound:
+  FLOOKUP (add_module_static_maps F src tls art).cta_flag_members k = SOME members ==>
+  FLOOKUP art.cta_flag_members k = SOME members \/
+  ?tl fid ls.
+    MEM tl tls /\ tl = FlagDecl fid ls /\ k = (src,fid) /\ members = ls
+Proof
+  qid_spec_tac `art` >> Induct_on `tls` >- rw[add_module_static_maps_def] >>
+  rw[add_module_static_maps_def] >>
+  first_x_assum (qspec_then `add_toplevel_static_maps F src h art` mp_tac) >>
+  simp[add_module_static_maps_def] >> strip_tac >-
+    (drule add_toplevel_static_maps_flag_members_sound >> rw[] >> gvs[] >> metis_tac[]) >>
+  metis_tac[]
+QED
+
+Theorem add_contract_static_maps_toplevel_vtypes_sound:
+  FLOOKUP (FOLDL (\art (src,tls). add_module_static_maps F src tls art) art mods).cta_toplevel_vtypes k = SOME vt ==>
+  FLOOKUP art.cta_toplevel_vtypes k = SOME vt \/
+  (?src tls tl vis mut id ty init.
+     MEM (src,tls) mods /\ MEM tl tls /\ tl = VariableDecl vis mut id ty init /\
+     k = (src,string_to_num id) /\ vt = Type ty) \/
+  (?src tls tl vis is_transient id kt vty init.
+     MEM (src,tls) mods /\ MEM tl tls /\ tl = HashMapDecl vis is_transient id kt vty init /\
+     k = (src,string_to_num id) /\ vt = HashMapT kt vty)
+Proof
+  qid_spec_tac `art` >> Induct_on `mods` >- rw[] >>
+  gen_tac >> PairCases_on `h` >> rw[] >>
+  first_x_assum (qspec_then `add_module_static_maps F h0 h1 art` mp_tac) >>
+  simp[] >> strip_tac >-
+    (drule add_module_static_maps_toplevel_vtypes_sound >> rw[] >> gvs[] >> metis_tac[]) >>
+  metis_tac[]
+QED
+
+Theorem add_contract_static_maps_bare_globals_sound:
+  FLOOKUP (FOLDL (\art (src,tls). add_module_static_maps F src tls art) art mods).cta_bare_globals k = SOME ty ==>
+  FLOOKUP art.cta_bare_globals k = SOME ty \/
+  (?src tls tl vis id typ init.
+     MEM (src,tls) mods /\ MEM tl tls /\ tl = VariableDecl vis Immutable id typ init /\
+     k = (src,string_to_num id) /\ ty = typ) \/
+  (?src tls tl vis e id typ init.
+     MEM (src,tls) mods /\ MEM tl tls /\ tl = VariableDecl vis (Constant e) id typ init /\
+     k = (src,string_to_num id) /\ ty = typ)
+Proof
+  qid_spec_tac `art` >> Induct_on `mods` >- rw[] >>
+  gen_tac >> PairCases_on `h` >> rw[] >>
+  first_x_assum (qspec_then `add_module_static_maps F h0 h1 art` mp_tac) >>
+  simp[] >> strip_tac >-
+    (drule add_module_static_maps_bare_globals_sound >> rw[] >> gvs[] >> metis_tac[]) >>
+  metis_tac[]
+QED
+
+Theorem add_contract_static_maps_bare_global_assignable_sound:
+  FLOOKUP (FOLDL (\art (src,tls). add_module_static_maps F src tls art) art mods).cta_bare_global_assignable k = SOME ty ==>
+  FLOOKUP art.cta_bare_global_assignable k = SOME ty \/
+  ?src tls tl vis id typ init.
+    MEM (src,tls) mods /\ MEM tl tls /\ tl = VariableDecl vis Immutable id typ init /\
+    k = (src,string_to_num id) /\ ty = typ
+Proof
+  qid_spec_tac `art` >> Induct_on `mods` >- rw[] >>
+  gen_tac >> PairCases_on `h` >> rw[] >>
+  first_x_assum (qspec_then `add_module_static_maps F h0 h1 art` mp_tac) >>
+  simp[] >> strip_tac >-
+    (drule add_module_static_maps_bare_global_assignable_sound >> rw[] >> gvs[] >> metis_tac[]) >>
+  metis_tac[]
+QED
+
+Theorem add_contract_static_maps_flag_members_sound:
+  FLOOKUP (FOLDL (\art (src,tls). add_module_static_maps F src tls art) art mods).cta_flag_members k = SOME members ==>
+  FLOOKUP art.cta_flag_members k = SOME members \/
+  ?src tls tl fid ls.
+    MEM (src,tls) mods /\ MEM tl tls /\ tl = FlagDecl fid ls /\
+    k = (src,fid) /\ members = ls
+Proof
+  qid_spec_tac `art` >> Induct_on `mods` >- rw[] >>
+  gen_tac >> PairCases_on `h` >> rw[] >>
+  first_x_assum (qspec_then `add_module_static_maps F h0 h1 art` mp_tac) >>
+  simp[] >> strip_tac >-
+    (drule add_module_static_maps_flag_members_sound >> rw[] >> gvs[] >> metis_tac[]) >>
+  metis_tac[]
+QED
+
+Theorem build_contract_type_artifact_toplevel_vtypes_sound:
+  contract_namespaces_ok F mods /\
+  FLOOKUP (build_contract_type_artifact F mods).cta_toplevel_vtypes (src,id) = SOME vt ==>
+  (?ts vis mut id_str ty init.
+     ALOOKUP mods src = SOME ts /\ MEM (VariableDecl vis mut id_str ty init) ts /\
+     id = string_to_num id_str /\ vt = Type ty) \/
+  (?ts vis is_transient id_str kt vty init.
+     ALOOKUP mods src = SOME ts /\ MEM (HashMapDecl vis is_transient id_str kt vty init) ts /\
+     id = string_to_num id_str /\ vt = HashMapT kt vty)
+Proof
+  rw[build_contract_type_artifact_def] >>
+  drule add_contract_static_maps_toplevel_vtypes_sound >> rw[] >> gvs[empty_contract_type_artifact_def] >>
+  gvs[] >> metis_tac[ALOOKUP_ALL_DISTINCT_MEM, contract_namespaces_ok_def]
+QED
+
+Theorem build_contract_type_artifact_bare_globals_sound:
+  contract_namespaces_ok F mods /\
+  FLOOKUP (build_contract_type_artifact F mods).cta_bare_globals (src,id) = SOME ty ==>
+  (?ts vis id_str init.
+     ALOOKUP mods src = SOME ts /\ MEM (VariableDecl vis Immutable id_str ty init) ts /\
+     id = string_to_num id_str) \/
+  (?ts vis e id_str init.
+     ALOOKUP mods src = SOME ts /\ MEM (VariableDecl vis (Constant e) id_str ty init) ts /\
+     id = string_to_num id_str)
+Proof
+  rw[build_contract_type_artifact_def] >>
+  drule add_contract_static_maps_bare_globals_sound >> rw[] >> gvs[empty_contract_type_artifact_def] >>
+  gvs[] >> metis_tac[ALOOKUP_ALL_DISTINCT_MEM, contract_namespaces_ok_def]
+QED
+
+Theorem build_contract_type_artifact_bare_global_assignable_sound:
+  contract_namespaces_ok F mods /\
+  FLOOKUP (build_contract_type_artifact F mods).cta_bare_global_assignable (src,id) = SOME ty ==>
+  ?ts vis id_str init.
+    ALOOKUP mods src = SOME ts /\ MEM (VariableDecl vis Immutable id_str ty init) ts /\
+    id = string_to_num id_str
+Proof
+  rw[build_contract_type_artifact_def] >>
+  drule add_contract_static_maps_bare_global_assignable_sound >> rw[] >> gvs[empty_contract_type_artifact_def] >>
+  qexistsl [`tls`,`vis`,`id'`,`init`] >> simp[] >>
+  metis_tac[ALOOKUP_ALL_DISTINCT_MEM, contract_namespaces_ok_def]
+QED
+
+Theorem flag_member_key_MEM:
+  MEM (FlagDecl fid members) ts ==>
+  MEM ((src : num option),fid) (FLAT (MAP (flag_member_keys_toplevel src) ts))
+Proof
+  rw[MEM_FLAT, MEM_MAP] >>
+  qexists `[(src,fid)]` >> simp[] >>
+  qexists `FlagDecl fid members` >>
+  simp[flag_member_keys_toplevel_def]
+QED
+
+Theorem lookup_flag_MEM_FlagDecl:
+  ALL_DISTINCT (FLAT (MAP (flag_member_keys_toplevel (src : num option)) ts)) /\
+  MEM (FlagDecl fid members) ts ==>
+  lookup_flag fid ts = SOME members
+Proof
+  Induct_on `ts` >- rw[lookup_flag_def] >>
+  gen_tac >> Cases_on `h` >>
+  rw[lookup_flag_def, flag_member_keys_toplevel_def] >>
+  gvs[lookup_flag_def, flag_member_keys_toplevel_def] >>
+  metis_tac[flag_member_key_MEM]
+QED
+
+Theorem contract_namespaces_ok_module_flag_member_keys:
+  contract_namespaces_ok F mods /\ MEM (src,tls) mods ==>
+  ALL_DISTINCT (FLAT (MAP (flag_member_keys_toplevel src) tls))
+Proof
+  rw[contract_namespaces_ok_def, contract_keys_def] >>
+  qpat_x_assum `ALL_DISTINCT (FLAT (MAP _ mods))` mp_tac >>
+  Induct_on `mods` >- rw[] >>
+  gen_tac >> PairCases_on `h` >> rw[] >> gvs[ALL_DISTINCT_APPEND]
+QED
+
+Theorem build_contract_type_artifact_flag_members_sound:
+  contract_namespaces_ok F mods /\
+  FLOOKUP (build_contract_type_artifact F mods).cta_flag_members (src,fid) = SOME members ==>
+  ?ts. ALOOKUP mods src = SOME ts /\ MEM (FlagDecl fid members) ts
+Proof
+  rw[build_contract_type_artifact_def] >>
+  drule add_contract_static_maps_flag_members_sound >> rw[] >> gvs[empty_contract_type_artifact_def] >>
+  qexists `tls` >> simp[] >>
+  irule ALOOKUP_ALL_DISTINCT_MEM >> gvs[contract_namespaces_ok_def] >> metis_tac[]
+QED
+
+(* The old same-source StructDecl/FlagDecl shadowing probe is intentionally not
+   kept as a theorem: checked contracts now reject such collisions via
+   type_def_keys_toplevel in contract_namespaces_ok. *)
+
+(* ===== Static-map completeness bridges for contract artifacts ===== *)
+
+Theorem check_contract_toplevel_vtypes_complete_initial:
+  check_contract F layouts addr mods = SOME art /\
+  ALOOKUP sources addr = SOME mods /\
+  tx.target = addr ==>
+  toplevel_vtypes_complete art.cta_toplevel_vtypes
+    (initial_evaluation_context sources layouts tx)
+Proof
+  cheat
+QED
+
+Theorem check_contract_bare_globals_complete_initial:
+  check_contract F layouts addr mods = SOME art /\
+  ALOOKUP sources addr = SOME mods /\
+  tx.target = addr ==>
+  bare_globals_complete art.cta_bare_globals
+    (initial_evaluation_context sources layouts tx)
+Proof
+  cheat
+QED
+
+Theorem check_contract_bare_global_assignable_complete_initial:
+  check_contract F layouts addr mods = SOME art /\
+  ALOOKUP sources addr = SOME mods /\
+  tx.target = addr ==>
+  bare_global_assignable_complete art.cta_bare_global_assignable
+    (initial_evaluation_context sources layouts tx)
+Proof
+  cheat
+QED
+
+Theorem check_contract_flag_members_complete_initial:
+  check_contract F layouts addr mods = SOME art /\
+  ALOOKUP sources addr = SOME mods /\
+  tx.target = addr ==>
+  flag_members_complete art.cta_flag_members
+    (initial_evaluation_context sources layouts tx)
+Proof
+  cheat
+QED
+
+(* ===== Static-map consistency bridges for contract artifacts ===== *)
+
+Theorem check_contract_bare_globals_consistent_initial:
+  check_contract F layouts addr mods = SOME art /\
+  ALOOKUP sources addr = SOME mods /\
+  tx.target = addr ==>
+  !src id ty.
+    FLOOKUP art.cta_bare_globals (src,id) = SOME ty ==>
+    ?ts. get_module_code (initial_evaluation_context sources layouts tx) src = SOME ts /\
+         FLOOKUP art.cta_toplevel_vtypes (src,id) = SOME (Type ty) /\
+         is_bare_global_decl id ts /\
+         find_var_decl_by_num id ts = NONE /\
+         ty <> NoneT
+Proof
+  cheat
+QED
+
+Theorem check_contract_bare_global_assignable_consistent_initial:
+  check_contract F layouts addr mods = SOME art /\
+  ALOOKUP sources addr = SOME mods /\
+  tx.target = addr ==>
+  !src id ty.
+    FLOOKUP art.cta_bare_global_assignable (src,id) = SOME ty ==>
+    ?ts. get_module_code (initial_evaluation_context sources layouts tx) src = SOME ts /\
+         FLOOKUP art.cta_bare_globals (src,id) = SOME ty /\
+         FLOOKUP art.cta_toplevel_vtypes (src,id) = SOME (Type ty) /\
+         is_immutable_decl id ts /\
+         find_var_decl_by_num id ts = NONE /\
+         ty <> NoneT
+Proof
+  cheat
+QED
+
+Theorem check_contract_toplevel_vtypes_consistent_initial:
+  check_contract F layouts addr mods = SOME art /\
+  ALOOKUP sources addr = SOME mods /\
+  tx.target = addr ==>
+  (!src id vt.
+     FLOOKUP art.cta_toplevel_vtypes (src,id) = SOME vt ==>
+     well_formed_vtype (type_env_all_modules mods) vt) /\
+  (!src id ty.
+     FLOOKUP art.cta_toplevel_vtypes (src,id) = SOME (Type ty) /\
+     FLOOKUP art.cta_bare_globals (src,id) = NONE ==>
+     ?ts is_transient typ id_str.
+       get_module_code (initial_evaluation_context sources layouts tx) src = SOME ts /\
+       find_var_decl_by_num id ts = SOME (StorageVarDecl is_transient typ,id_str) /\
+       typ = ty /\
+       IS_SOME (evaluate_type (type_env_all_modules mods) typ) /\
+       IS_SOME (lookup_var_slot_from_layout
+         (initial_evaluation_context sources layouts tx) is_transient src id_str)) /\
+  (!src id kt vt.
+     FLOOKUP art.cta_toplevel_vtypes (src,id) = SOME (HashMapT kt vt) ==>
+     ?ts is_transient id_str.
+       get_module_code (initial_evaluation_context sources layouts tx) src = SOME ts /\
+       find_var_decl_by_num id ts = SOME (HashMapVarDecl is_transient kt vt,id_str) /\
+       IS_SOME (lookup_var_slot_from_layout
+         (initial_evaluation_context sources layouts tx) is_transient src id_str))
+Proof
+  cheat
+QED
+
+Theorem check_contract_flag_members_consistent_initial:
+  check_contract F layouts addr mods = SOME art /\
+  ALOOKUP sources addr = SOME mods /\
+  tx.target = addr ==>
+  !src fid ls.
+    FLOOKUP art.cta_flag_members (src,fid) = SOME ls ==>
+    ?ts. get_module_code (initial_evaluation_context sources layouts tx) src = SOME ts /\
+         lookup_flag fid ts = SOME ls /\
+         FLOOKUP (type_env_all_modules mods) (type_key (src,fid)) =
+           SOME (FlagArgs (LENGTH ls))
+Proof
+  cheat
+QED
+
+(* ===== Env-context bridge for initial contexts ===== *)
+
+Theorem check_contract_env_context_consistent_initial_NONE:
+  check_contract F layouts addr mods = SOME art /\
+  ALOOKUP sources addr = SOME mods /\
+  tx.target = addr ==>
+  env_context_consistent (artifact_env art mods NONE)
+    (initial_evaluation_context sources layouts tx)
+Proof
+  rw[env_context_consistent_def, artifact_env_def]
+  >- simp[get_tenv_def, initial_evaluation_context_def]
+  >- simp[current_module_def, initial_evaluation_context_def]
+  >- (irule check_contract_fn_sigs_consistent_initial >> simp[])
+  >- (irule check_contract_fn_sigs_complete_initial >> simp[])
+  >- (irule check_contract_toplevel_vtypes_complete_initial >> simp[])
+  >- (irule check_contract_bare_globals_complete_initial >> simp[])
+  >- (irule check_contract_bare_global_assignable_complete_initial >> simp[])
+  >- (irule check_contract_flag_members_complete_initial >> simp[])
+  >- metis_tac[check_contract_bare_globals_consistent_initial]
+  >- (dxrule check_contract_bare_global_assignable_consistent_initial >>
+      simp[] >> disch_then (qspecl_then [`src`,`id`,`ty`] mp_tac) >> simp[])
+  >- (dxrule check_contract_toplevel_vtypes_consistent_initial >>
+      simp[] >> disch_then (qspecl_then [`tx`,`sources`] mp_tac) >>
+      simp[] >> strip_tac >> metis_tac[])
+  >- (dxrule check_contract_toplevel_vtypes_consistent_initial >>
+      simp[] >> disch_then (qspecl_then [`tx`,`sources`] mp_tac) >>
+      simp[get_tenv_def, initial_evaluation_context_def] >> strip_tac >> metis_tac[])
+  >- (dxrule check_contract_toplevel_vtypes_consistent_initial >>
+      simp[] >> disch_then (qspecl_then [`tx`,`sources`] mp_tac) >>
+      simp[] >> strip_tac >> metis_tac[])
+  >- (dxrule check_contract_flag_members_consistent_initial >>
+      simp[] >> strip_tac >>
+      first_x_assum (qspecl_then [`tx`,`sources`,`src`,`fid`,`ls`] mp_tac) >>
+      simp[get_tenv_def, initial_evaluation_context_def])
+QED
+
+Theorem get_tenv_stk[local]:
+  !cx stk. get_tenv (cx with stk := stk) = get_tenv cx
+Proof
+  simp[get_tenv_def]
+QED
+
+Theorem get_module_code_stk[local]:
+  !cx stk src. get_module_code (cx with stk := stk) src = get_module_code cx src
+Proof
+  simp[get_module_code_def]
+QED
+
+Theorem lookup_var_slot_from_layout_stk[local]:
+  !cx stk is_transient src id.
+    lookup_var_slot_from_layout (cx with stk := stk) is_transient src id =
+    lookup_var_slot_from_layout cx is_transient src id
+Proof
+  simp[lookup_var_slot_from_layout_def]
+QED
+
+Theorem fn_sigs_consistent_stk[local]:
+  !sigs cx stk.
+    fn_sigs_consistent sigs (cx with stk := stk) <=> fn_sigs_consistent sigs cx
+Proof
+  simp[fn_sigs_consistent_def, get_module_code_stk]
+QED
+
+Theorem fn_sigs_complete_stk[local]:
+  !sigs cx stk.
+    fn_sigs_complete sigs (cx with stk := stk) <=> fn_sigs_complete sigs cx
+Proof
+  simp[fn_sigs_complete_def, get_module_code_stk]
+QED
+
+Theorem toplevel_vtypes_complete_stk[local]:
+  !m cx stk.
+    toplevel_vtypes_complete m (cx with stk := stk) <=>
+    toplevel_vtypes_complete m cx
+Proof
+  simp[toplevel_vtypes_complete_def, get_module_code_stk]
+QED
+
+Theorem bare_globals_complete_stk[local]:
+  !m cx stk.
+    bare_globals_complete m (cx with stk := stk) <=> bare_globals_complete m cx
+Proof
+  simp[bare_globals_complete_def, get_module_code_stk]
+QED
+
+Theorem bare_global_assignable_complete_stk[local]:
+  !m cx stk.
+    bare_global_assignable_complete m (cx with stk := stk) <=>
+    bare_global_assignable_complete m cx
+Proof
+  simp[bare_global_assignable_complete_def, get_module_code_stk]
+QED
+
+Theorem flag_members_complete_stk[local]:
+  !m cx stk.
+    flag_members_complete m (cx with stk := stk) <=> flag_members_complete m cx
+Proof
+  simp[flag_members_complete_def, get_module_code_stk]
+QED
+
+Theorem check_contract_env_context_consistent_initial_with_current_src:
+  check_contract F layouts addr mods = SOME art /\
+  ALOOKUP sources addr = SOME mods /\
+  tx.target = addr ==>
+  env_context_consistent (artifact_env art mods src)
+    ((initial_evaluation_context sources layouts tx) with stk := [(src, fn)])
+Proof
+  rw[env_context_consistent_def, artifact_env_def]
+  >- simp[get_tenv_stk, get_tenv_def, initial_evaluation_context_def]
+  >- simp[current_module_def]
+  >- (simp[fn_sigs_consistent_stk] >>
+      irule check_contract_fn_sigs_consistent_initial >> simp[])
+  >- (simp[fn_sigs_complete_stk] >>
+      irule check_contract_fn_sigs_complete_initial >> simp[])
+  >- (simp[toplevel_vtypes_complete_stk] >>
+      irule check_contract_toplevel_vtypes_complete_initial >> simp[])
+  >- (simp[bare_globals_complete_stk] >>
+      irule check_contract_bare_globals_complete_initial >> simp[])
+  >- (simp[bare_global_assignable_complete_stk] >>
+      irule check_contract_bare_global_assignable_complete_initial >> simp[])
+  >- (simp[flag_members_complete_stk] >>
+      irule check_contract_flag_members_complete_initial >> simp[])
+  >- (dxrule check_contract_bare_globals_consistent_initial >>
+      simp[] >> strip_tac >>
+      first_x_assum (qspecl_then [`tx`,`sources`,`src'`,`id`,`ty`] mp_tac) >>
+      simp[get_module_code_stk])
+  >- (dxrule check_contract_bare_global_assignable_consistent_initial >>
+      simp[] >> strip_tac >>
+      first_x_assum (qspecl_then [`tx`,`sources`,`src'`,`id`,`ty`] mp_tac) >>
+      simp[get_module_code_stk])
+  >- (dxrule check_contract_toplevel_vtypes_consistent_initial >>
+      simp[] >> disch_then (qspecl_then [`tx`,`sources`] mp_tac) >>
+      simp[] >> strip_tac >> metis_tac[])
+  >- (dxrule check_contract_toplevel_vtypes_consistent_initial >>
+      simp[] >> disch_then (qspecl_then [`tx`,`sources`] mp_tac) >>
+      simp[get_tenv_stk, get_tenv_def, initial_evaluation_context_def,
+           get_module_code_stk, lookup_var_slot_from_layout_stk] >>
+      strip_tac >> metis_tac[])
+  >- (dxrule check_contract_toplevel_vtypes_consistent_initial >>
+      simp[] >> disch_then (qspecl_then [`tx`,`sources`] mp_tac) >>
+      simp[get_module_code_stk, lookup_var_slot_from_layout_stk] >>
+      strip_tac >> metis_tac[])
+  >- (dxrule check_contract_flag_members_consistent_initial >>
+      simp[] >> strip_tac >>
+      first_x_assum (qspecl_then [`tx`,`sources`,`src'`,`fid`,`ls`] mp_tac) >>
+      simp[get_tenv_stk, get_tenv_def, initial_evaluation_context_def,
+           get_module_code_stk])
+QED
